Add: 補題

theories/Equivalence.v
@@ -12,6 +12,36 @@ Declare ML Module "ltac_plugin".
 Set Default Proof Mode "Classic".
 
 
+Definition retraction_idmap
+  {A : Type}
+  : @retraction A A idmap idmap .
+Proof.
+ refine (fun x => _) .
+ unfold compose, idmap .
+ exact (idpath x) .
+Defined.
+
+Definition section_idmap
+  {A : Type}
+  : @section A A idmap idmap .
+Proof.
+ refine (fun x => _) .
+ unfold compose, idmap .
+ exact (idpath x) .
+Defined.
+
+Definition is_adjoint_idmap
+  {A : Type}
+  : @is_adjoint A A idmap idmap retraction_idmap section_idmap .
+Proof.
+ refine (fun x => _) .
+ unfold pwpaths_compose10, pwpaths_compose01 .
+ unfold compose10, compose01 .
+ unfold retraction_idmap, section_idmap .
+ unfold compose_dep, ap, paths_elim_nodep .
+ exact (idpath (idpath x)) .
+Defined.
+
 Definition is_equiv_idmap {A : Type} : is_equiv (@idmap A) .
 Proof.
  refine (dpair idmap _) .
@@ -32,4 +62,3 @@ Definition is_equiv_compose
   : is_equiv (compose g f) .
 Proof.
  refine (dpair (compose (equiv_inv f_iv) (equiv_inv g_iv)) _) .
- 
